graphs conform to algos, correctness-completeness lemmas for each step

theories/dfs_xleroy/dfs_inloop.v
@@ -9,31 +9,19 @@
 (*         CeCILL v2.1 FREE SOFTWARE LICENSE AGREEMENT        *)
 (**************************************************************)
 
-(* TODO: remove this comment
-   Work in progress: consistency with [2] and the other files
-   of the current directory
-   DONE: accumulator at the end everywhere, Gfoldleft instead of iterel
-   TODO: use only Braga_book techniques
- *)
-
 (* The Braga method applied to dfs, expressed with an internal loop *)
-(* Jean-François Monin, Verimag, Univ. Grenoble-Alpes, 2024         *)
 
 (* Using ideas coming from
 [1] Xavier Leroy, Well-founded recursion done right, CoqPL 2024
     https://inria.hal.science/hal-04356563/document
 [2] Dominique Larchey-Wendling and Jean-François Monin
     The Braga Method https://cnrs.hal.science/hal-03338785v1
-[3] Jean-François Monin, Smaller Inversions and Unleashed Recursion in Coq (talk)
-    https://www-verimag.imag.fr/~monin/Talks/sir.pdf
 
 The algorithm provided in [1] is not quite the usual dfs algorithm
 Chapter 1 shows the use of the Braga method on the rectified version
 of this algorithm.
 Then Chapter 2 provides a number of transformations from
 this algorithm to the one considered in [2].
-
-We use small inversions explained in [3].
 
  *)
 
@@ -45,9 +33,7 @@ Import ListNotations.
 #[local] Infix "∉" := (λ x a, ¬ In x a) (at level 70, no associativity).
 
 Require Import dfs_abstract.
-
-(* Gfoldleft is convenient for dfs_stack.
-   Then we reuse it for Gdfs_list as well (but keep Ddfs_list mutual recursive) *)
+Arguments Gfl_nil {X Y F a}.
 
 (* Reminder
 Inductive Gfoldleft (X Y : Type) (F : Y → X → X → Prop) : list Y → X → X → Prop :=
@@ -59,28 +45,18 @@ Inductive Gfoldleft (X Y : Type) (F : Y → X → X → Prop) : list Y → X →
 (* Small inversion of Gfoldleft *)
 Inductive Gfoldleft_nil {X Y : Type} (R : Y → X → X → Prop) (a : X) : X → Prop :=
 | Gfl_nil_nil : Gfoldleft_nil R a a.
-Inductive Gfoldleft_cons {X Y : Type} (R : Y → X → X → Prop) y l (a : X) : X → Prop :=
-| Gfl_cons_cons b c : R y a b → Gfoldleft R l b c → Gfoldleft_cons R y l a c.
+Inductive Gfoldleft_cons {X Y : Type} (R : Y → X → X → Prop) y l (a : X) (c : X) : Prop :=
+| Gfl_cons_cons b : R y a b → Gfoldleft R l b c → Gfoldleft_cons R y l a c.
 Definition Gfoldleft_dispatch {X Y} (R : Y → X → X → Prop) l a : X → Prop :=
   match l with
   | [] => Gfoldleft_nil R a
   | y :: l => Gfoldleft_cons R y l a
   end.
 
-Lemma Gfoldleft_inv {X Y : Type} {R : Y → X → X → Prop}
+Definition Gfoldleft_inv {X Y : Type} {R : Y → X → X → Prop}
   {a l b} (i : Gfoldleft R l a b) : Gfoldleft_dispatch R l a b.
-Proof. destruct i; econstructor; eassumption. Qed.
+Proof. destruct i; econstructor; eassumption. Defined.
 (* End of small inversion *)
-
-(* TODO Diterel? *)
-
-Lemma Gfoldleft_first {X Y} (R : Y → X → X → Prop) y1 {y2 a l b} :
-  (R y1 a ⊆ R y2 a) → Gfoldleft R (y1 :: l) a b → Gfoldleft R (y2 :: l) a b.
-Proof.
-  intros rr i.
-  destruct (Gfoldleft_inv i) as [b c r i0].
-  apply (Gfl_cons (rr _ r) i0).
-Qed.
 
 Section dfs.
 
@@ -125,45 +101,92 @@ Section dfs.
      tend to be decomposed into annoying "knitting/unknitting" steps
        let   (result, postcond) := terminal_recursive_call in
        exist result new_postcond
-    Additional penalty : the Coq code is then no longer tail recursive.
-    Considering extraction this is harmless since the extraction process is smart
-    enough to recover tail recursion through a clever optimization step.
-    However we show below a way to keep terminal recursivity at the Coq level
-    using a propositional continuation.
+     Additional penalty : the Coq code is then no longer tail recursive.
+     Considering extraction this is harmless since the extraction process is smart
+     enough to recover tail recursion through a clever optimization step.
+     However we show below a way to keep terminal recursivity at the Coq level
+     using a propositional continuation.
 
-    We try make the intended (OCaml) functional algorithm as apparent as possible,
-    as well as structurally decreasing terms.
-    For (proofs of) postconditions, a possible technique is to use the [refine]
-    tactic, with jokers for postconditions.
-    See for example the sibling file dfs_xleroy.v by Dominique.
-    However the management of postconditions turns out to be quite simple
-    in the present framework -- basically, constructors of the i/o relation.
-    Here we choose to provide fully explicit terms, using greek letters
-    for propositional arguments and ad-hoc spacing for better readibility.
+     We try make the intended (OCaml) functional algorithm as apparent as possible,
+     as well as structurally decreasing terms.
+     For (proofs of) postconditions, a possible technique is to use the [refine]
+     tactic, with jokers for postconditions.
+     See for example the sibling file dfs_xleroy.v by Dominique.
+     However the management of postconditions turns out to be quite simple
+     in the present framework -- basically, constructors of the i/o relation.
+     Here we choose to provide fully explicit terms, using greek letters
+     for propositional arguments and ad-hoc spacing for better readibility.
 
-    An additional interest of the sibling file dfs_xleroy.v is to formalize
-    and experiment a partial version of List.fold_left, of independent interest.
-    (Here we stick to mutual recursion, as in [1].)
-    Extraction seems to behave better with mutual recursion -- no silent
-    unused argument is introduced.
+     An additional interest of the sibling file dfs_xleroy.v is to formalize
+     and experiment a partial version of List.fold_left, of independent interest.
+     (Here we stick to mutual recursion, as in [1].)
+     Extraction seems to behave better with mutual recursion -- no silent
+     unused argument is introduced.
  *)
 
   Inductive Gdfs : X → list X → list X → Prop :=
-  | Gdfs_stop {a x} :     x ∈ a
+  | Gdfs_stop {x a} :     x ∈ a
                         → Gdfs x a a
-  | Gdfs_next {a x o} :   x ∉ a
-                        → Gfoldleft Gdfs (succs x) (x :: a) o
-                        → Gdfs x a o.
+  | Gdfs_next {x a o} :   x ∉ a
+                        → Gdfs_list (succs x) (x :: a) o
+                        → Gdfs x a o
+  with Gdfs_list : list X → list X → list X → Prop :=
+  | Gdl_nil {a} :            Gdfs_list [] a a
+  | Gdl_cons {x l a b o} :   Gdfs x a b
+                           → Gdfs_list l b o
+                           → Gdfs_list (x :: l) a o.
 
-  Definition Gdfs_list : list X → list X → list X → Prop := Gfoldleft Gdfs.
+  Definition Gdfs_main := λ x, Gdfs x [].
 
-  Definition Gdfs_simple := λ x, Gdfs x [].
+  (* Small inversion of Gdfs_list *)
+  Inductive Gdfs_list_nil (a : list X) : list X → Prop :=
+  | Gdl_nil_nil : Gdfs_list_nil a a.
+  Inductive Gdfs_list_cons x l (a : list X) (o : list X) : Prop :=
+  | Gdl_cons_cons b : Gdfs x a b → Gdfs_list l b o → Gdfs_list_cons x l a o.
+  Definition Gdfs_list_dispatch l a : list X → Prop :=
+    match l with
+    | []     => Gdfs_list_nil a
+    | x :: l => Gdfs_list_cons x l a
+    end.
+
+  Definition Gdfs_list_inv {l a o} (γ : Gdfs_list l a o) : Gdfs_list_dispatch l a o.
+  Proof. destruct γ; econstructor; eassumption. Defined.
+  (* End of small inversion *)
+
+
+  Lemma Gdfs_deterministic {x a o} (γ : Gdfs x a o) : ∀ {o'}, Gdfs x a o' → o = o'.
+  Proof.
+    revert x a o γ.
+    refine (fix loop1 x a o γ {struct γ} : _ := _).
+    destruct γ as [x a yes | x a o no γ]; intros o' γ'.
+    - destruct γ' as [x a _ | x a o no γ']; [reflexivity | case (no yes)].
+    - destruct γ' as [x a yes | x a o' _ γ']; [case (no yes) | clear no; revert o' γ'].
+      refine (
+          let fix loop2 l a o (γ : Gdfs_list l a o) {struct γ} : ∀ o', Gdfs_list l a o' → o = o' := _
+          in loop2 (succs x) (x :: a) o γ).
+      destruct γ as [a | x' l a b o γab γbo e]; intros o' γ'.
+      + destruct (Gdfs_list_inv γ'). reflexivity.
+      + destruct (Gdfs_list_inv γ') as [b' γab' γb'o'].
+        apply (loop2 _ _ _ γbo).
+        rewrite (loop1 x' a b γab b' γab').
+        exact γb'o'.
+  Qed.
+
+  Definition Gdfs_list_corr {x a o} : Gdfs_list [x] a o → Gdfs x a o.
+  Proof.
+    intro γ.
+    destruct (Gdfs_list_inv γ) as [b γab γbo]; destruct (Gdfs_list_inv γbo).
+    exact γab.
+  Defined.
+
+  Definition Gdfs_list_compl {x a o} : Gdfs x a o → Gdfs_list [x] a o
+    := λ γ, Gdl_cons γ Gdl_nil.
 
   (* Corresponding inductive domain, but mutual recursive *)
   Inductive Ddfs : X → list X → Prop :=
-  | Ddfs_stop {a x} :     x ∈ a
+  | Ddfs_stop {x a} :     x ∈ a
                         → Ddfs x a
-  | Ddfs_next {a x} :     x ∉ a
+  | Ddfs_next {x a} :     x ∉ a
                         → Ddfs_list (succs x) (x :: a)
                         → Ddfs x a
 
@@ -213,45 +236,19 @@ Section dfs.
           match l                                         (* *) return Ddfs_list l a -> _
           with
           | [] =>                                         (* *) λ _,
-                  exist a                                 (* *) (Gfl_nil a)
+                  exist a                                 (* *) Gdl_nil
           | y :: l =>                                     (* *) λ δ,
               let (b, γab) := dfs y a                     (* *) (Ddfs_list_cons_pi1 δ)
                                                           (* *) in let δ := Ddfs_list_cons_pi2 δ b γab
               in let (o, γbo) := dfs_list l b             (* *) δ
-              in exist o                                  (* *) (Gfl_cons γab γbo)
+              in exist o                                  (* *) (Gdl_cons γab γbo)
           end                                             (* *) δ
         in let (o, γ) := dfs_list (succs x) (x :: a)      (* *) (Ddfs_next_pi δ no)
         in exist o                                        (* *) (Gdfs_next no γ)
     end.
 
   (* Main program: the inlined nested variant of dfs_cycle *)
-  Definition dfs_cycle_inld x : Ddfs x [] → {o | Gdfs x [] o} := dfs x [].
-
-  (* Elimination of (un-)knitting steps; intended tail-recursive calls are recovered *)
-    Fixpoint dfs_tr (x: X) (a: list X)       (* *) (δ: Ddfs x a) {struct δ}
-    : {o | Gdfs x a o} :=
-    match in_dec x a with
-    | left yes => exist a                    (* *) (Gdfs_stop yes)
-    | right no =>
-                                             (* *) let post o := Gdfs x a o (* keeps the global a *)
-        in let fix dfs_list l a              (* *) (δ : Ddfs_list l a) {struct δ}
-             :                               (* *) (∀ o, Gdfs_list l a o → post o) →
-               {o | post o} :=
-          match l                            (* *) return Ddfs_list l a -> _
-          with
-          | [] =>                            (* *) λ _ κ,
-                  exist a                    (* *) (κ a (@Gfl_nil _ _ Gdfs a)) (*Gfl_nil a*)
-          | y :: l =>                        (* *) λ δ κ,
-              let (b, γab) := dfs_tr y a     (* *) (Ddfs_list_cons_pi1 δ)
-                                             (* *) in let δ := Ddfs_list_cons_pi2 δ b γab
-                                             (* *) in let κ := λ o γbo, κ o (Gfl_cons γab γbo)
-              in dfs_list l b                (* *) δ κ
-          end                                (* *) δ
-        in dfs_list (succs x) (x :: a)       (* *) (Ddfs_next_pi δ no) (λ o g, Gdfs_next no g)
-    end.
-
-  (* Main *)
-  Definition dfs_cycle_inld_tr x : Ddfs x [] → {o | Gdfs x [] o} := dfs_tr x [].
+  Definition dfs_cycle_inld x : Ddfs x [] → {o | Gdfs_main x o} := dfs x [].
 
   (* Chapter 2. Derivation of fully tail-recursive algorithms, including the one in [2] *)
 
@@ -259,85 +256,123 @@ Section dfs.
 
   (* Rearrangement of dfs_list above, where the call to dfs is inlined *)
 
-  (* Ad-hoc versions of Gdfs etc. could be defined, but the previous ones
-     can be re-used. Then there is no need to prove equivalence between
-   specifications.  *)
+  Inductive Gdfs_list_self : list X → list X → list X → Prop :=
+  | Gdls_nil {a} :               Gdfs_list_self [] a a
+  | Gdls_cons_yes {x l a o} :    x ∈ a
+                               → Gdfs_list_self l a o
+                               → Gdfs_list_self (x :: l) a o
+  | Gdls_cons_no {x l a b o} :   x ∉ a
+                               → Gdfs_list_self (succs x) (x :: a) b
+                               → Gdfs_list_self l b o
+                               → Gdfs_list_self (x :: l) a o.
 
-  Lemma Gdfs_singleton {a x o} : x ∉ a → Gdfs_list [x] a o → Gdfs x a o.
+  Inductive Ddfs_list_self : list X → list X → Prop :=
+  | Ddls_nil {a} :        Ddfs_list_self [] a
+  | Ddls_cons_yes [x l a] :   x ∈ a
+                            → Ddfs_list_self l a
+                            → Ddfs_list_self (x :: l) a
+  | Ddls_cons_no  [x l a] :   x ∉ a
+                            → Ddfs_list_self (succs x) (x :: a)
+                            → (∀ b, Gdfs_list_self (succs x) (x :: a) b → Ddfs_list_self l b)
+                            → Ddfs_list_self (x :: l) a.
+
+  Definition Ddfs_list_self_cons_yes_pi {x l a} (δ : Ddfs_list_self (x :: l) a) :
+    x ∈ a → Ddfs_list_self l a :=
+    match δ in Ddfs_list_self xl a return
+          let shape := match xl with x :: l => True | _ => False end in
+          let x :=     match xl with x :: l => x    | _ => x end in
+          let l :=     match xl with x :: l => l    | _ => l end in
+          shape → x ∈ a → Ddfs_list_self l a
+    with
+    | Ddls_cons_yes _ δ => λ sh yes, δ
+    | Ddls_cons_no no _ _ => λ sh yes, match no yes with end
+    | _ => λ sh yes, match sh with end
+    end I.
+
+  Definition Ddfs_list_self_cons_no_pi1 {x l a} (δ : Ddfs_list_self (x :: l) a) :
+    x ∉ a → Ddfs_list_self (succs x) (x :: a) :=
+    match δ in Ddfs_list_self xl a return
+          let shape := match xl with x :: l => True | _ => False end in
+          let x :=     match xl with x :: l => x    | _ => x end in
+          let l :=     match xl with x :: l => l    | _ => l end in
+          shape → x ∉ a → Ddfs_list_self (succs x) (x :: a)
+    with
+    | Ddls_cons_no _ δ1 fδ2 => λ sh no, δ1
+    | Ddls_cons_yes yes _ => λ sh no, match no yes with end
+    | _ => λ sh no, match sh with end
+    end I.
+
+  Definition Ddfs_list_self_cons_no_pi2 {x l a} (δ : Ddfs_list_self (x :: l) a) :
+    x ∉ a → (∀ b, Gdfs_list_self (succs x) (x :: a) b → Ddfs_list_self l b) :=
+    match δ in Ddfs_list_self xl a return
+          let shape := match xl with x :: l => True | _ => False end in
+          let x :=     match xl with x :: l => x    | _ => x end in
+          let l :=     match xl with x :: l => l    | _ => l end in
+          shape → x ∉ a → (∀ b, Gdfs_list_self (succs x) (x :: a) b → Ddfs_list_self l b)
+    with
+    | Ddls_cons_no _ δ1 fδ2 => λ sh no, fδ2
+    | Ddls_cons_yes yes _ => λ sh no, match no yes with end
+    | _ => λ sh no, match sh with end
+    end I.
+
+  Fixpoint dfs_list_self l a                      (* *) (δ : Ddfs_list_self l a) {struct δ}
+    : {o | Gdfs_list_self l a o}  :=
+    match l                                       (* *) return Ddfs_list_self l a -> _
+    with
+    | [] =>                                       (* *) λ _,
+        exist a                                   (* *) Gdls_nil
+    | x :: l =>                                   (* *) λ δ,
+        match in_dec x a with
+        | left yes =>                             (* *) let δ := Ddfs_list_self_cons_yes_pi δ yes in
+            let (o, γao) := dfs_list_self l a     (* *) δ
+            in exist o                            (* *) (Gdls_cons_yes yes γao)
+        | right no =>                             (* *) let δ1 := Ddfs_list_self_cons_no_pi1 δ no in
+            let (b, γab) := dfs_list_self (succs x) (x :: a)
+                                                  (* *) δ1
+                                                  (* *) in let δ2 := Ddfs_list_self_cons_no_pi2 δ no b γab
+            in let (o, γbo) := dfs_list_self l b  (* *) δ2
+            in exist o                            (* *) (Gdls_cons_no no γab γbo)
+          end
+    end                                           (* *) δ.
+
+  (* Main *)
+  Definition dfs_cycle_self x                     (* *) (δ : Ddfs_list_self [x] [])
+    : {o | Gdfs_list_self [x] [] o} :=
+    dfs_list_self [x] []                          (* *) δ.
+
+  (* Correctness and completeness of Gdfs_list_self / Gdfs_list*)
+  Lemma Gdfs_list_self_corr {l a o} :
+    Gdfs_list_self l a o → Gdfs_list l a o.
   Proof.
-    intros no γ. apply (Gdfs_next no).
-    destruct (Gfoldleft_inv γ) as [b o γab γbo]; clear γ.
-    destruct (Gfoldleft_inv γbo); clear γbo.
-    destruct γab as [a x yes | a x b _no γ]; [case (no yes) | exact γ].
+    intro γ. induction γ as [a | x a l o yes γ Hγ | x a b l o no γab Hγab γbo Hγbo].
+    - constructor.
+    - exact (Gdl_cons (Gdfs_stop yes) Hγ).
+    - exact (Gdl_cons (Gdfs_next no Hγab) Hγbo).
   Qed.
 
-  Lemma Gdfs_singleton_nil {x o} : Gdfs_list [x] [] o → Gdfs x [] o.
-  Proof. exact (λ γ, Gdfs_singleton (λ (absu : x ∈ []), absu) γ). Qed.
+  Fixpoint Gdfs_list_self_compl_cons {x a l b} (γ : Gdfs x a b) {struct γ} :
+    ∀ {o}, Gdfs_list_self l b o → Gdfs_list_self (x :: l) a o.
+  Proof.
+    destruct γ as [x ac yes | x a b no γ]; intros o γbo.
+    - apply (Gdls_cons_yes yes), γbo.
+    - refine (Gdls_cons_no no _ γbo).
+      induction γ as [a0 | x0 l0 a0 c b γa0c γcb Hγcb].
+      + constructor.
+      + exact (Gdfs_list_self_compl_cons x0 a0 l0 c γa0c b (Hγcb γbo)).
+  Qed.
 
-  Fixpoint dfs_list_self l a                  (* *) (δ : Ddfs_list l a) {struct δ}
-    : {o | Gdfs_list l a o}  :=
-    match l                                   (* *) return Ddfs_list l a -> _
-    with
-    | [] =>                                   (* *) λ _,
-        exist a                               (* *) (Gfl_nil a)
-    | x :: l =>                               (* *) λ δ,
-        let (b, γab) :=
-          match in_dec x a with
-          | left yes => exist a               (* *) (Gdfs_stop yes)
-          | right no =>
-                                              (* *) let δ := Ddfs_list_cons_pi1 δ
-                                              (* *) in let δ := Ddfs_next_pi δ no
-              in let (o, γ) := dfs_list_self (succs x) (x :: a)
-                                              (* *) δ
-              in exist o                      (* *) (Gdfs_next no γ)
-          end
-                                              (* *) in let δ := Ddfs_list_cons_pi2 δ b γab
-        in let (o, γbo) := dfs_list_self l b  (* *) δ
-        in exist o                            (* *) (Gfl_cons γab γbo)
-    end                                       (* *) δ.
-
-  (* Main *)
-  Definition dfs_cycle_self x                 (* *) (δ : Ddfs x [])
-    : {o | Gdfs x [] o} :=
-                                              (* *) let δ := Ddfs_list_cons δ (λ b _, Ddfs_list_nil)
-    in let (o, γ) := dfs_list_self [x] []     (* *) δ
-    in exist o                                (* *) (Gdfs_singleton_nil γ).
-
-  (* Elimination of (un-)knitting steps:
-     an additional parameter for post is needed in the (internal) dfs_listk *)
-  Fixpoint dfs_list_self_tr
-                        l a                (* *) (δ : Ddfs_list l a) {struct δ}
-    :                                      (* *) ∀ (post : list X → Prop), (∀ o, Gdfs_list l a o → post o) →
-      {o | post o} :=
-                                           (* *) λ post,
-    match l                                (* *) return Ddfs_list l a → _
-    with
-    | [] =>                                (* *) λ _ κ,
-        exist a                            (* *) (κ a (@Gfl_nil _ _ Gdfs a))
-    | x :: l =>                            (* *) λ δ κ,
-      let (b, γab) :=
-          match in_dec x a with
-          | left yes => exist a            (* *) (Gdfs_stop yes)
-          | right no =>
-                                           (* *) let δ := Ddfs_list_cons_pi1 δ
-                                           (* *) in let δ := Ddfs_next_pi δ no
-            in dfs_list_self_tr (succs x) (x :: a)
-                                           (* *) δ (Gdfs x a) (λ o γ, Gdfs_next no γ)
-          end
-                                           (* *) in let δ := Ddfs_list_cons_pi2 δ b γab
-      in dfs_list_self_tr l b                  (* *) δ post (λ o γbo, κ o (Gfl_cons γab γbo))
-    end                                    (* *) δ.
-
-  (* Main *)
-  Definition dfs_cycle_self_tr x           (* *) (δ : Ddfs x [])
-    : {o | Gdfs x [] o} :=
-                                           (* *) let δ := Ddfs_list_cons δ (λ b _, Ddfs_list_nil)
-    in dfs_list_self_tr [x] []             (* *) δ (Gdfs x []) (λ o γ, Gdfs_singleton_nil γ).
+  Lemma Gdfs_list_self_compl {l a o} :
+    Gdfs_list l a o → Gdfs_list_self l a o.
+  Proof.
+    intro γ; induction γ as [a | x a l b c γab γbc Hγbc].
+    - constructor.
+    - exact (Gdfs_list_self_compl_cons γab Hγbc).
+  Qed.
 
   (* 2.2 Elimination of embedded recursion using a stack s *)
 
   (* Two versions can be considered.
-  The first one looks closer to dfs_list in dfs_self above.
+  The first one looks closer to dfs_list_self above.
   let dfs =
     let rec dfs_list_stack l s a =
       match l with
@@ -423,48 +458,98 @@ Section dfs.
 
   (* *)
 
-  Inductive Gdfs_stack : stack X → list X → list X → Prop :=
-  | Gdfs_stack_nil {a} :                 Gdfs_stack [] a a
-  | Gdfs_stack_nil_emp {a} :             Gdfs_stack ([] :: []) a a
-  | Gdfs_stack_nil_push {l s a o}  :     Gdfs_stack (l :: s) a o
-                                       → Gdfs_stack ([] :: l :: s) a o
-  | Gdfs_stack_cons_stop {x l s a o} :   x ∈ a
-                                       → Gdfs_stack (l :: s) a o
-                                       → Gdfs_stack ((x :: l) :: s) a o
-  | Gdfs_stack_cons_next {x l s a o} :   x ∉ a
-                                       → Gdfs_stack (succs x :: l :: s) (x :: a) o
-                                       → Gdfs_stack ((x :: l) :: s) a o.
+  Inductive Gdfs_list_stack : list X → stack X → list X → list X → Prop :=
+  | Gls_nil_emp {a} :             Gdfs_list_stack [] [] a a
+  | Gls_nil_push {l s a o}  :     Gdfs_list_stack l s a o
+                                → Gdfs_list_stack [] (l :: s) a o
+  | Gls_cons_stop {x l s a o} :   x ∈ a
+                                → Gdfs_list_stack l s a o
+                                → Gdfs_list_stack (x :: l) s a o
+  | Gls_cons_next {x l s a o} :   x ∉ a
+                                → Gdfs_list_stack (succs x) (l :: s) (x :: a) o
+                                → Gdfs_list_stack (x :: l) s a o.
 
-  Definition Gdfs_stack_list: list X → stack X → list X → list X → Prop :=
-    λ l s, Gdfs_stack (l :: s).
-
-  Fixpoint dfs_list_stack l s a (δ : Ddfs_stack (l :: s) a) {struct δ} : {o | Gdfs_stack_list l s a o} :=
+  Fixpoint dfs_list_stack l s a (δ : Ddfs_stack (l :: s) a) {struct δ} : {o | Gdfs_list_stack l s a o} :=
     match l                                                             (* *) return Ddfs_stack (l :: s) a → _
     with
     | [] =>                                                             (* *) λ δ,
         match s                                                         (* *) return Ddfs_stack ([] :: s) a → _
         with
         | []     =>                                                     (* *) λ _,
-                    exist a                                             (* *) Gdfs_stack_nil_emp
+                    exist a                                             (* *) Gls_nil_emp
         | l :: s =>                                                     (* *) λ δ,
                     let (o, γ) := dfs_list_stack l s a                  (* *) (Ddfs_stack_nil_push_pi δ)
-                    in exist o                                          (* *) (Gdfs_stack_nil_push γ)
+                    in exist o                                          (* *) (Gls_nil_push γ)
         end                                                             (* *) δ
     | x :: l =>                                                         (* *) λ δ,
         match in_dec x a with
         | left yes =>
                     let (o, γ) := dfs_list_stack l s a                  (* *) (Ddfs_stack_cons_stop_pi δ yes)
-                    in exist o                                          (* *) (Gdfs_stack_cons_stop yes γ)
+                    in exist o                                          (* *) (Gls_cons_stop yes γ)
         | right no =>
                     let (o, γ) := dfs_list_stack (succs x) (l :: s) (x :: a)
                                                                         (* *) (Ddfs_stack_cons_next_pi δ no)
-                    in exist o                                          (* *) (Gdfs_stack_cons_next no γ)
+                    in exist o                                          (* *) (Gls_cons_next no γ)
         end
     end δ.
 
   (* Main *)
   Definition dfs_cycle_stack x :                                        (* *)  Ddfs_stack ([x] :: []) [] →
-                                 {o | Gdfs_stack_list [x] [] [] o} := dfs_list_stack [x] [] [].
+                                 {o | Gdfs_list_stack [x] [] [] o} := dfs_list_stack [x] [] [].
+
+  (* Specification and correctness of dfs_list_stack / Gdfs_list_self *)
+
+  Definition Gdfs_list_self_star := Gfoldleft Gdfs_list_self.
+
+  Inductive Gdfs_list_self_plus l s a o : Prop :=
+  | Gls_plus b :   Gdfs_list_self l a b → Gdfs_list_self_star s b o
+                 → Gdfs_list_self_plus l s a o.
+  Arguments Gls_plus {l s a o}.
+
+  Lemma Gdfs_list_stack_corr {l s a o} :   Gdfs_list_stack l s a o
+                                         → Gdfs_list_self_plus l s a o.
+  Proof.
+    induction 1 as [a | l s a o γ Hγ
+                   | x l s a o yes γ Hγ
+                   | x l s a o no γ Hγ].
+    - exact (Gls_plus a Gdls_nil Gfl_nil).
+    - exact (let (b, γab, γbo) := Hγ in Gls_plus a Gdls_nil (Gfl_cons γab γbo)).
+    - exact (let (b, γab, γbo) := Hγ in Gls_plus b (Gdls_cons_yes yes γab) γbo).
+    - exact (let (b, γxab, γbo) := Hγ in
+             let (c, γbc, γco) := Gfoldleft_inv γbo in
+             Gls_plus c (Gdls_cons_no no γxab γbc) γco).
+  Qed.
+
+  (* ------------------------------------------------------------------------------------------ *)
+  (* dfs_stack *)
+
+  Inductive Gdfs_stack : stack X → list X → list X → Prop :=
+  | Gs_nil {a} :          Gdfs_stack [] a a
+  | Gs_cons {l s a o} :   Gdfs_list_stack l s a o
+                        → Gdfs_stack (l :: s) a o.
+
+  (* Fake constructors for Gdfs_stack *)
+  Definition promote {l s a o l' s' a' o'} (f : Gdfs_list_stack l s a o → Gdfs_list_stack l' s' a' o') :
+    Gdfs_stack (l :: s) a o → Gdfs_stack (l' :: s') a' o'.
+    refine (λ γ, Gs_cons (f match γ in Gdfs_stack ls a o return
+                                  match ls with l :: s => Gdfs_list_stack l s a o | _ => IDProp end
+                            with
+                            | Gs_cons γ => γ
+                            | _ => idProp
+                            end)).
+  Defined.
+
+  Definition Gs_nil_push {l s a o}  :     Gdfs_stack (l :: s) a o
+                                        → Gdfs_stack ([] :: l :: s) a o
+    := promote Gls_nil_push.
+  Definition Gs_cons_stop {x l s a o} :   x ∈ a
+                                        → Gdfs_stack (l :: s) a o
+                                        → Gdfs_stack ((x :: l) :: s) a o
+    := λ yes, promote (Gls_cons_stop yes).
+  Definition Gs_cons_next {x l s a o} :    x ∉ a
+                                         → Gdfs_stack (succs x :: l :: s) (x :: a) o
+                                         → Gdfs_stack ((x :: l) :: s) a o
+    := λ no, promote (Gls_cons_next no).
 
   (* *)
 
@@ -472,18 +557,18 @@ Section dfs.
     match s                                                                 (* *) return Ddfs_stack s a → _
     with
     | []     =>                                                             (* *) λ _,
-              exist a                                                       (* *) Gdfs_stack_nil
+              exist a                                                       (* *) Gs_nil
     | [] :: [] =>                                                           (* *) λ δ,
-              exist a                                                       (* *) Gdfs_stack_nil_emp
+              exist a                                                       (* *) (Gs_cons Gls_nil_emp)
     | [] :: s =>                                                            (* *) λ δ,
               let (o, γ) := dfs_stack s a                                   (* *) (Ddfs_stack_nil_push_pi δ)
-              in exist o                                                    (* *) (Gdfs_stack_nil_push γ)
+              in exist o                                                    (* *) (Gs_nil_push γ)
     | (x :: l) :: s =>                                                      (* *) λ δ,
         match in_dec x a with
         | left yes => let (o, γ) := dfs_stack (l :: s) a                    (* *) (Ddfs_stack_cons_stop_pi δ yes)
-                      in exist o                                            (* *) (Gdfs_stack_cons_stop yes γ)
+                      in exist o                                            (* *) (Gs_cons_stop yes γ)
         | right no => let (o, γ) := dfs_stack (succs x :: l :: s) (x :: a)  (* *) (Ddfs_stack_cons_next_pi δ no)
-                      in exist o                                            (* *) (Gdfs_stack_cons_next no γ)
+                      in exist o                                            (* *) (Gs_cons_next no γ)
         end
     end δ.
 
@@ -491,198 +576,92 @@ Section dfs.
   Definition dfs_book_eff x :                                               (* *)  Ddfs_stack ([[x]]) [] →
                               {o | Gdfs_stack [[x]] [] o} := dfs_stack [[x]] [].
 
+  (* Specification and correctness of dfs_stack / dfs_list_stack *)
+
+  Definition Gdfs_stack_corr {l s a o} :   Gdfs_stack (l :: s) a o
+                                         → Gdfs_list_stack l s a o
+    := λ γ, match γ in Gdfs_stack ls a o return
+                  match ls with l :: s => Gdfs_list_stack l s a o | _ => IDProp end
+            with
+            | Gs_cons γ => γ
+            | _ => idProp
+            end.
+
+  (* not really useful? *)
+  Corollary Gdfs_stack_corr_list_self {s a o} :   Gdfs_stack s a o
+                                                → Gdfs_list_self_star s a o.
+  Proof.
+    destruct 1 as [a | l s a o γ].
+    - apply Gfl_nil.
+    - destruct (Gdfs_list_stack_corr γ) as [b γab γbo]. exact (Gfl_cons γab γbo).
+  Qed.
+
   (* Specification and correctness of dfs_list_stack / Gdfs *)
 
   Definition Gdfs_list_star := Gfoldleft Gdfs_list.
 
   Inductive Gdfs_list_plus l s a o : Prop :=
-  | Gdfs_list_plus_in b :   Gdfs_list l a b
-                          → Gdfs_list_star s b o
-                          → Gdfs_list_plus l s a o.
+  | Gl_plus b :   Gdfs_list l a b → Gdfs_list_star s b o
+                → Gdfs_list_plus l s a o.
 
-  (* From Gdfs_list_star to Gdfs_simple *)
+  (* From Gdfs_list_star to Gdfs_main *)
 
-  Lemma Gdfs_list_star_Gdfs x o : Gdfs_list_star [[x]] [] o → Gdfs_simple x o.
+  Lemma Gdfs_list_star_Gdfs x o : Gdfs_list_star [[x]] [] o → Gdfs_main x o.
   Proof.
     intro γxo.
-    destruct (Gfoldleft_inv γxo) as [c o γxc γco]; destruct (Gfoldleft_inv γco); clear γxo γco.
-    destruct (Gfoldleft_inv γxc) as [b c γxb γbc]; destruct (Gfoldleft_inv γbc); clear γxc γbc.
+    destruct (Gfoldleft_inv γxo) as [c γxc γco]; destruct (Gfoldleft_inv γco); clear γxo γco.
+    destruct (Gdfs_list_inv γxc) as [b γxb γbc]; destruct (Gdfs_list_inv γbc); clear γxc γbc.
     exact γxb.
   Qed.
 
+  (* .......................................................................... *)
+
+  (* Completeness of Gdfs_stack wrt Gdfs, Gdfs_list[star, plus] *)
+  (* Easy fake constructor for Gdfs_list_stack *)
+
+  (* Key lemma *)
+  Lemma list_self_cont_stack {l a b} (γab : Gdfs_list_self l a b) :
+    ∀ {s o}, Gdfs_list_stack [] s b o → Gdfs_list_stack l s a o.
+  Proof.
+    induction γab as [a | x l a b yes γab Hγab | x l a b c no γxab Hγxab γbc Hγbc];
+      intros s o γ.
+    - exact γ.
+    - exact (Gls_cons_stop yes (Hγab s o γ)).
+    - exact (Gls_cons_next no (Hγxab (l :: s) o (Gls_nil_push (Hγbc s o γ)))).
+  Qed.
+
+  Lemma Gdfs_list_stack_compl_nil {s a o} :   Gdfs_list_self_star s a o
+                                            → Gdfs_list_stack [] s a o.
+  Proof.
+    induction 1 as [a | l a s b o γab _ γbo].
+    - exact Gls_nil_emp.
+    - apply Gls_nil_push. exact (list_self_cont_stack γab γbo).
+  Qed.
+
+  Lemma Gdfs_list_stack_compl {l s a o} :   Gdfs_list_self_plus l s a o
+                                          → Gdfs_list_stack l s a o.
+  Proof.
+    intros [b γab γbo]. revert s γbo.
+    induction γab as [ a | x l a b yes γab Hγab | x l a b c no γxab Hγxab γbc Hγbc]; intros s γ.
+    - exact (Gdfs_list_stack_compl_nil γ).
+    - exact (Gls_cons_stop yes (Hγab s γ)).
+    - exact (Gls_cons_next no (Hγxab _ (Gfl_cons γbc γ))).
+  Qed.
+
+
+
   (* *)
 
-  Fact Gdfs_list_plus_corr1 a :
-    Gdfs_list_plus [] [] a a.
-  Proof.
-    exists a; exact (Gfl_nil a).
-  Qed.
+  Lemma Gdfs_stack_compl {l s a o} :
+    Gdfs_list_stack l s a o → Gdfs_stack (l :: s) a o.
+  Proof. intro γ. exact (Gs_cons γ). Qed.
 
-  Fact Gdfs_list_plus_corr2 {l s a o} :
-      Gdfs_list_plus l s a o
-    → Gdfs_list_plus [] (l :: s) a o.
-  Proof.
-    destruct 1 as [b γab γbo].
-    exists a; [exact (Gfl_nil a) | exact (Gfl_cons γab γbo)].
-  Qed.
-
-  Fact Gdfs_list_plus_corr3 {x l s a o} (yes : x ∈ a) :
-      Gdfs_list_plus l s a o
-    → Gdfs_list_plus (x :: l) s a o.
-  Proof.
-    destruct 1 as [b γab γbo].
-    exists b; [exact (Gfl_cons (Gdfs_stop yes) γab) | exact γbo].
-  Qed.
-
-  Fact Gdfs_list_plus_corr4 {x l s a o} (no : x ∉ a) :
-      Gdfs_list_plus (succs x) (l :: s) (x :: a) o
-    → Gdfs_list_plus (x :: l) s a o.
-  Proof.
-    destruct 1 as [b γxab γbo].
-    destruct (Gfoldleft_inv γbo) as [c o γbc γco].
-    exists c; [exact (Gfl_cons (Gdfs_next no γxab) γbc) | exact γco].
-  Qed.
-
-  Lemma Gdfs_list_stack_corr {l s a o} :   Gdfs_stack_list l s a o
-                                        → Gdfs_list_plus l s a o.
-  Proof.
-    revert l s; intros l0 s0 γ;
-    change (match l0 :: s0 with
-            | [] => True
-            | l :: s => Gdfs_list_plus l s a o
-            end);
-    induction γ as [a | a | l s a o γ Hγ
-                   | x l s a o yes γ Hγ
-                   | x l s a o no γ Hγ]; clear l0 s0.
-    - exact I.
-    - apply Gdfs_list_plus_corr1.
-    - apply Gdfs_list_plus_corr2, Hγ.
-    - apply (Gdfs_list_plus_corr3 yes), Hγ.
-    - apply (Gdfs_list_plus_corr4 no), Hγ.
-  Qed.
-
-  Lemma Gdfs_list_stack_compl l s a o :   Gdfs_list_plus l s a o
-                                        → Gdfs_stack_list l s a o.
-  Proof.
-    intros [b γab γbo]. red.
-    (* Pas si facile ; peut-être faire dfs_stack_compl avant *)
-  Abort.
-    (*
-    revert o γbo.
-    induction γab as [ a | x a l b o γab _ γbo].
-    - intros o γbo.
-      induction γbo as [ a | l a s b o γab γ γbo].
-      + constructor.
-      + apply (Gdfs_stack_nil_push).
-      induction s as [ | l s Hs].
-      + destruct (Gfoldleft_inv γbo). constructor.
-      + apply (Gdfs_stack_nil_push). γbo).
-    - induction γab as [ a | x a l b o γab _ γbo].
-      + constructor.
-      + destruct γab as [a x yes | a x b no γxab].
-        * exact (Gdfs_stack_cons_stop yes γbo).
-        * apply (Gdfs_stack_cons_next no). admit.
-*)
-
-   (*
-  (* ---------------------------------------------------------------------- *)
-  (* Recursive equations of dfs_stack *)
-  Fact dfs_stack_eqn0 {a} (δ : Ddfs_stack [] a) : dfs_stack [] a δ = a.
-  Proof. destruct (Ddfs_stack_inv δ); cbn. reflexivity. Qed.
-
-  Fact dfs_stack_eqn1 {a} (δ : Ddfs_stack [[]] a) : dfs_stack [[]] a δ = a.
-  Proof. destruct (Ddfs_stack_inv δ); cbn. reflexivity. Qed.
-
-  Fact dfs_stack_eqn2 {l s a} (δ : Ddfs_stack ([] :: l :: s) a) :
-    dfs_stack ([] :: l :: s) a δ = dfs_stack (l :: s) a (Ddfs_stack_nil_push_pi δ).
-  Proof. destruct (Ddfs_stack_inv δ); cbn. reflexivity. Qed.
-
-  Fact dfs_stack_eqn3 {x l s a} (yes : x ∈ a) (δ : Ddfs_stack ((x :: l) :: s) a) :
-    dfs_stack ((x :: l) :: s) a δ = dfs_stack (l :: s) a (Ddfs_stack_cons_stop_pi δ yes).
-  Proof.
-    destruct (Ddfs_stack_inv δ) as [yes' δ | no δ]; cbn.
-    - destruct (in_dec x a) as [_ | no].
-      + reflexivity.
-      + case (no yes).
-    - case (no yes).
-  Qed.
-
-  Fact dfs_stack_eqn4 {x l s a} (no : x ∉ a) (δ : Ddfs_stack ((x :: l) :: s) a) :
-    dfs_stack ((x :: l) :: s) a δ =
-    dfs_stack (succs x :: l :: s) (x :: a) (Ddfs_stack_cons_next_pi δ no).
-   Proof.
-     destruct (Ddfs_stack_inv δ) as [yes δ | no' δ]; cbn.
-     - case (no yes).
-     - destruct (in_dec x a) as [yes | _].
-      + case (no yes).
-      + reflexivity.
-   Qed.
-*)
-
-  (* dfs_list_stack is a special case of dfs_stack
-   Lemma dfs_list_stack_same {l s a} (δ δ' : Ddfs_stack (l :: s) a) :
-     dfs_stack (l :: s) a δ = dfs_list_stack l s a δ'. *)
-  (* Semble couvert par Gdfs_stack_list l s := Gdfs_stack (l :: s) *)
-
-  (* Corollaire amusant : dfs_list_stack ne dépend pas de δ *)
-  (* TODO determinisme de dfs_list_stack *)
-(*   Corollary dfs_list_stack_domirr l s a (δ δ' : Ddfs_stack (l :: s) a) :
-     dfs_list_stack l s a δ = dfs_list_stack l s a δ'.
-   Proof.
-     rewrite <- (dfs_list_stack_same δ δ), <-(dfs_list_stack_same δ δ').
-     reflexivity.
-   Qed.
-*)
+  (* TODO use or remove or explain relevance *)
   Definition Ddfs_stack_nil_l {s a} : Ddfs_stack s a → Ddfs_stack ([] :: s) a :=
     match s with
     | [] => λ _, Ddfs_stack_nil_emp
     | l :: s => λ δ, (Ddfs_stack_nil_push δ)
     end.
-
-  Lemma Gdfs_stack_case {s a o} (γ : Gdfs_stack s a o) :
-    match s with [] => a = o | l :: s => Gdfs_stack_list l s a o end.
-  Proof.
-    destruct γ as [a | a | l s a o γ
-                     | x l s a o yes γ
-                     | x l s a o no γ]; try red.
-    - reflexivity.
-    - apply Gdfs_stack_nil_emp.
-    - exact (Gdfs_stack_nil_push γ).
-    - exact (Gdfs_stack_cons_stop yes γ).
-    - exact (Gdfs_stack_cons_next no γ).
-  Qed.
-
-  (* A correctness proof of dfs_stack using correctness of dfs_list_stack / Gdfs *)
-
-  Lemma Gdfs_stack_corr {s a o} :   Gdfs_stack s a o
-                                  → Gdfs_list_star s a o.
-  Proof.
-    intro γ. generalize (Gdfs_stack_case γ).
-    destruct s as [ | l s]; clear γ; intro γ.
-    - case γ. apply Gfl_nil.
-    - destruct (Gdfs_list_stack_corr γ) as [b γab γbo]. exact (Gfl_cons γab γbo).
-  Qed.
-
-  (*
-  (* TODO cmplétude ? *)
-  Lemma Gdfs_stack_compl {s a o} :   Gdfs_list_star s a o
-                                   → Gdfs_stack s a o.
-  Proof.
-    induction 1 as [ a | l a s c o γac _ γco].
-    - apply Gdfs_stack_nil.
-    - revert o γco.
-      induction γac as [ a | x a l b c γab γbc' fcb]; intros o γco.
-      + generalize (Gdfs_stack_case γco).
-        destruct s as [ | l s]; clear γco; intro γco.
-        * case γco. apply Gdfs_stack_nil_emp.
-        * exact (Gdfs_stack_nil_push γco).
-      +
-        destruct γab as [ a x yes | a x b no γxab].
-        * apply (Gdfs_stack_cons_stop yes). apply fcb, γco.
-        * apply (Gdfs_stack_cons_next no).
-          Check (fcb o γco).
-
-*)
 
    (* 2.3 Flattening s in dfs_stack provides the algorithm considered in [2] *)
 
@@ -765,18 +744,6 @@ Section dfs.
 
   (* Relating dfs_flatten with dfs_stack *)
 
-  Remark Gdfs_stack_nil_all {s a o} : Gdfs_stack s a o → Gdfs_stack ([] :: s) a o.
-  Proof.
-    destruct 1 as [a | a | l s a o γ
-                   | x l s a o yes γ
-                   | x l s a o no  γ ]; cbn; try apply Gdfs_stack_nil_push.
-    - apply Gdfs_stack_nil_emp.
-    - apply Gdfs_stack_nil_emp.
-    - apply (Gdfs_stack_nil_push γ).
-    - apply (Gdfs_stack_cons_stop yes γ).
-    - apply (Gdfs_stack_cons_next no γ).
-  Qed.
-
   (* An inductive characterization of flatten in the spirit of Gdfs_stack *)
   Inductive iflatten : list (list X) → list X → Prop :=
   | ifl_nil : iflatten [] []
@@ -791,9 +758,6 @@ Section dfs.
     - induction l as [ | x l Hl]; now constructor.
   Qed.
 
-  Corollary iflatten_flatten_eq {s ls} : flatten s = ls → iflatten s ls.
-  Proof. intro e. case e. apply iflatten_flatten. Qed.
-
   Lemma flatten_iflatten {s ls} : iflatten s ls → flatten s = ls.
   Proof.
     intro ifl. induction ifl as [ | s ls ifl Hifl | s x l ls ifl Hifl]; cbn.
@@ -805,7 +769,9 @@ Section dfs.
   Corollary iflatten_app {s ls l} : iflatten s ls → iflatten (l :: s) (l ++ ls).
   Proof. intro ifl. case (flatten_iflatten ifl). apply iflatten_flatten. Qed.
 
-  (* Recursive small inversion of iflatten on its second argument *)
+  (* Recursive small inversion of iflatten on its second argument;
+     recursion is performed only on the ifl_cons_nil clause,
+     dedicated to the cancelation of empty elements in the stack *)
   Inductive iflatten_nil : list (list X) → Prop :=
   | ifln_nil : iflatten_nil []
   | ifln_cons_nil {s} : iflatten_nil s → iflatten_nil ([] :: s).
@@ -826,114 +792,106 @@ Section dfs.
   Qed.
   (* End of small inversion *)
 
+  Remark Gdfs_list_stack_nil_all {s a o} : Gdfs_stack s a o → Gdfs_list_stack [] s a o.
+  Proof.
+    destruct 1 as [a | l s a o γ].
+    - apply Gls_nil_emp.
+    - apply (Gls_nil_push γ).
+  Qed.
+  Remark Gdfs_stack_nil_all {s a o} : Gdfs_stack s a o → Gdfs_stack ([] :: s) a o.
+  Proof.
+    intro γ. apply Gs_cons, Gdfs_list_stack_nil_all, γ.
+  Qed.
+
   Lemma Gdfs_iflatten_corr {s a o ls} :
     Gdfs_flatten ls a o → iflatten s ls → Gdfs_stack s a o.
   Proof.
-    intros γ ifl. generalize (iflatten_inv ifl). clear ifl. revert s.
+    intros γ ifl. generalize (iflatten_inv ifl); clear ifl. revert s.
     induction γ as [ a | x ls a o yes γ Hγ | x ls a o no γ Hγ]; cbn; intros s ifl.
-    - induction ifl as [ s | s ifl Hifl].
-      + apply Gdfs_stack_nil.
+    - induction ifl as [ | s ifl Hifl].
+      + apply Gs_nil.
       + apply Gdfs_stack_nil_all. apply Hifl.
     - induction ifl as [ s ifl Hifl | l s ifl].
       + apply Gdfs_stack_nil_all. apply Hifl.
-      + apply (Gdfs_stack_cons_stop yes), Hγ, iflatten_inv, ifl.
+      + apply (Gs_cons_stop yes), Hγ, iflatten_inv, ifl.
     - induction ifl as [ s ifl Hifl | l s ifl].
       + apply Gdfs_stack_nil_all. apply Hifl.
-      + apply (Gdfs_stack_cons_next no), Hγ, iflatten_inv.
+      + apply (Gs_cons_next no), Hγ, iflatten_inv.
         apply iflatten_app, ifl.
   Qed.
 
   (* *)
 
-  Lemma Gdfs_flatten_corr_eq {s a o ls} :
-    Gdfs_flatten ls a o → flatten s = ls → Gdfs_stack s a o.
-  Proof.
-    intros γ e. exact (Gdfs_iflatten_corr γ (iflatten_flatten_eq e)).
-  Qed.
-
   Corollary Gdfs_flatten_corr {s a o} :
     Gdfs_flatten (flatten s) a o → Gdfs_stack s a o.
-  Proof. intro γ. apply (Gdfs_flatten_corr_eq γ eq_refl). Qed.
+  Proof. exact (λ γ, Gdfs_iflatten_corr γ (iflatten_flatten s)). Qed.
 
+  (* Completeness of Gdfs_flatten / Gdfs_stack is much easier *)
   Lemma Gdfs_flatten_compl {s a o} :
     Gdfs_stack s a o → Gdfs_flatten (flatten s) a o.
   Proof.
-    induction 1 as [a | a | l s a o γ Hγ
+    destruct 1 as [a | l s a o γ]; cbn.
+    - exact Gdfs_flatten_nil.
+    - induction γ as [a | l s a o γ Hγ
                    | x l s a o yes γ Hγ
-                   | x l s a o no γ Hγ]; cbn.
-    - constructor.
-    - constructor.
-    - exact Hγ.
-    - apply (Gdfs_flatten_cons_stop yes Hγ).
-    - apply (Gdfs_flatten_cons_next no Hγ).
+                     | x l s a o no γ Hγ]; cbn.
+      + exact Gdfs_flatten_nil.
+      + exact Hγ.
+      + exact (Gdfs_flatten_cons_stop yes Hγ).
+      + exact (Gdfs_flatten_cons_next no Hγ).
   Qed.
 
-  (* Small inversion Gdfs_flatten *)
+  (* ----------------------------------------------------------------------- *)
+  (* Correctness and completeness of Gdfs_stack and Gdfs_flatten / Gdfs_list *)
+  (* By chaining the previous lemmas, taking an initial singleton stack.     *)
 
-  Inductive Gdfs_flatten_part_nil : list X → list X → Prop :=
-  | Gdfs_flatten_part_nil_nil {a} :                  Gdfs_flatten_part_nil a a.
-  Inductive Gdfs_flatten_part_cons x ls : list X → list X → Prop :=
-  | Gdfs_flatten_part_cons_stop {a o} :     x ∈ a
-                                          → Gdfs_flatten ls a o
-                                          → Gdfs_flatten_part_cons x ls a o
-  | Gdfs_flatten_part_cons_next {a o} :     x ∉ a
-                                          → Gdfs_flatten (succs x ++ ls) (x :: a) o
-                                          → Gdfs_flatten_part_cons x ls a o.
-  Definition Gdfs_flatten_dispatch (ls : list X) : list X → list X → Prop :=
-    match ls with
-    | []      => Gdfs_flatten_part_nil
-    | x :: ls => Gdfs_flatten_part_cons x ls
-    end.
-  Definition Gdfs_flatten_inv {ls a o} (γ : Gdfs_flatten ls a o) : Gdfs_flatten_dispatch ls a o.
-  Proof. destruct γ; constructor; assumption. Qed.
-  (* End of small inversion *)
+  Fact Gplus1_intro {l a o} : Gdfs_list_self l a o → Gdfs_list_self_plus l [] a o.
+  Proof. exact (λ γ, Gls_plus _ γ Gfl_nil). Qed.
 
-  Lemma dfs_flatten_same {s a o o'} :
-    Gdfs_stack s a o → Gdfs_flatten (flatten s) a o' → o = o'.
+  Fact Gplus1_elim {l a o} : Gdfs_list_self_plus l [] a o → Gdfs_list_self l a o.
+  Proof. destruct 1 as [b γab γbo]. destruct (Gfoldleft_inv γbo). exact γab. Qed.
+
+  Fact flatten1 {l} : flatten [l] = l.
+  Proof. apply app_nil_r. Qed.
+
+  (* *)
+
+  Lemma Gdfs_stack_corr_list {l a o} : Gdfs_stack [l] a o → Gdfs_list l a o.
   Proof.
-    induction 1 as [a | a | l s a o γ Hγ
-                   | x l s a o yes γ Hγ
-                   | x l s a o no γ Hγ]; cbn; intro γ'.
-    - destruct (Gdfs_flatten_inv γ') as [a]. reflexivity.
-    - destruct (Gdfs_flatten_inv γ') as [a]. reflexivity.
-    - cbn in Hγ. generalize γ'. destruct γ' as [ a | x ls a o' yes | x ls a o' no]; try clear γ'.
-      + exact Hγ.
-      + exact Hγ.
-      + exact Hγ.
-   - destruct (Gdfs_flatten_inv γ') as [a o' _ γ'0 | a o' no _ ].
-      + apply (Hγ γ'0).
-      + case (no yes).
-   - destruct (Gdfs_flatten_inv γ') as [a o' yes _ | a o' _ γ'0 ].
-      + case (no yes).
-      + exact (Hγ γ'0).
+    intro γ. apply Gdfs_list_self_corr, Gplus1_elim, Gdfs_list_stack_corr, Gdfs_stack_corr, γ.
   Qed.
 
-  Ltac unflatten := repeat (change (?l ++ flatten ?s) with (flatten (l :: s))).
-
-  Definition Ddfs_stack_flatten {a s} (δ : Ddfs_stack s a) : Ddfs_flatten (flatten s) a.
+  Lemma Gdfs_stack_compl_list {l a o} : Gdfs_list l a o → Gdfs_stack [l] a o.
   Proof.
-    refine ( (fix loop s a (δ : Ddfs_stack s a) {struct δ}: _ := _) s a δ).
-    destruct δ as [a | a | l s a | x l s a yes δ | x l s a no δ]; cbn; unflatten.
-    - constructor.
-    - constructor.
-    - apply loop, δ.
-    - apply (Ddfs_flatten_cons_stop yes), loop, δ.
-    - apply (Ddfs_flatten_cons_next no). unflatten. apply loop, δ.
-  Defined.
+    intro γ. apply Gdfs_stack_compl, Gdfs_list_stack_compl, Gplus1_intro, Gdfs_list_self_compl, γ.
+  Qed.
 
-  Lemma Gdfs_flatten_Gdfs {s a o} :
-    Gdfs_flatten (flatten s) a o → Gdfs_list_star s a o.
-  Proof. intro γ. apply Gdfs_stack_corr. apply (Gdfs_flatten_corr γ). Qed.
+  Lemma Gdfs_flatten_corr_list {l a o} : Gdfs_flatten l a o → Gdfs_list l a o.
+  Proof.
+    intro γ; apply Gdfs_stack_corr_list, Gdfs_flatten_corr.
+    rewrite flatten1. exact γ.
+  Qed.
 
-  (* Correctness of dfs_book_eff and dfs_book / Gdfs *)
+  Lemma Gdfs_flatten_compl_list {l a o} : Gdfs_list l a o → Gdfs_flatten l a o.
+  Proof.
+    intro γ;  rewrite <- flatten1.
+    apply Gdfs_flatten_compl, Gdfs_stack_compl_list, γ.
+  Qed.
 
-  Corollary Gdfs_book_eff_Gdfs {x o} :
-    Gdfs_stack [[x]] [] o → Gdfs_simple x o.
-  Proof. intro γ. apply Gdfs_list_star_Gdfs, Gdfs_stack_corr, γ. Qed.
+  (* Correctness and completeness of dfs_book_eff and dfs_book / Gdfs *)
 
-  Corollary dfs_book_Gdfs {x o} :
-    Gdfs_flatten [x] [] o → Gdfs_simple x o.
-  Proof. intro γ. apply Gdfs_book_eff_Gdfs, Gdfs_flatten_corr, γ. Qed.
+  Corollary Gdfs_book_eff_corr {x o} : Gdfs_stack [[x]] [] o → Gdfs_main x o.
+  Proof. exact (λ γ, Gdfs_list_corr (Gdfs_stack_corr_list γ)). Qed.
+
+  Corollary Gdfs_book_eff_compl {x o} : Gdfs_main x o → Gdfs_stack [[x]] [] o.
+  Proof. exact (λ γ, Gdfs_stack_compl_list (Gdfs_list_compl γ)). Qed.
+
+  Corollary Gdfs_book_Gdfs {x o} : Gdfs_flatten [x] [] o → Gdfs_main x o.
+  Proof. exact (λ γ, Gdfs_list_corr (Gdfs_flatten_corr_list γ)). Qed.
+
+  Corollary Gdfs_book_compl {x o} : Gdfs_main x o → Gdfs_flatten [x] [] o.
+  Proof. exact (λ γ, Gdfs_flatten_compl_list (Gdfs_list_compl γ)). Qed.
+
 
 End dfs.
 
